theories/sta_weak.v
@@ -6,27 +6,27 @@ Set Implicit Arguments.
 Unset Strict Implicit.
 Unset Printing Implicit Defensive.
 
-Inductive agree_ren : (var -> var) ->
+Inductive sta_agree_ren : (var -> var) ->
   sta_ctx term -> sta_ctx term -> Prop :=
-| agree_ren_nil ξ :
-  agree_ren ξ nil nil
-| agree_ren_cons Γ Γ' ξ m :
-  agree_ren ξ Γ Γ' ->
-  agree_ren (upren ξ) (m :: Γ) (m.[ren ξ] :: Γ')
-| agree_ren_wk Γ Γ' ξ m :
-  agree_ren ξ Γ Γ' ->
-  agree_ren (ξ >>> (+1)) (Γ) (m :: Γ').
+| sta_agree_ren_nil ξ :
+  sta_agree_ren ξ nil nil
+| sta_agree_ren_cons Γ Γ' ξ m :
+  sta_agree_ren ξ Γ Γ' ->
+  sta_agree_ren (upren ξ) (m :: Γ) (m.[ren ξ] :: Γ')
+| sta_agree_ren_wk Γ Γ' ξ m :
+  sta_agree_ren ξ Γ Γ' ->
+  sta_agree_ren (ξ >>> (+1)) (Γ) (m :: Γ').
 
-Lemma agree_ren_refl Γ : agree_ren id Γ Γ.
-Proof with eauto using agree_ren.
+Lemma sta_agree_ren_refl Γ : sta_agree_ren id Γ Γ.
+Proof with eauto using sta_agree_ren.
   elim: Γ...
   move=>A Γ ih.
-  have:(agree_ren (upren id) (A :: Γ) (A.[ren id] :: Γ))...
+  have:(sta_agree_ren (upren id) (A :: Γ) (A.[ren id] :: Γ))...
   by asimpl.
 Qed.
 
-Lemma agree_ren_sta_has Γ Γ' ξ x A :
-  agree_ren ξ Γ Γ' -> sta_has Γ x A -> sta_has Γ' (ξ x) A.[ren ξ].
+Lemma sta_agree_ren_has Γ Γ' ξ x A :
+  sta_agree_ren ξ Γ Γ' -> sta_has Γ x A -> sta_has Γ' (ξ x) A.[ren ξ].
 Proof with eauto.
   move=>agr. elim: agr x A=>{Γ Γ' ξ}.
   { move=>ξ x A hs. inv hs. }
@@ -41,12 +41,12 @@ Proof with eauto.
 Qed.
 
 Lemma sta_rename Γ Γ' m A ξ :
-  Γ ⊢ m : A -> agree_ren ξ Γ Γ' -> Γ' ⊢ m.[ren ξ] : A.[ren ξ].
-Proof with eauto using sta_type, agree_ren.
+  Γ ⊢ m : A -> sta_agree_ren ξ Γ Γ' -> Γ' ⊢ m.[ren ξ] : A.[ren ξ].
+Proof with eauto using sta_type, sta_agree_ren.
   move=>ty. elim: ty Γ' ξ=>{Γ m A}...
   { move=>Γ x A hs Γ' ξ agr. asimpl.
     apply: sta_var.
-    apply: agree_ren_sta_has... }
+    apply: sta_agree_ren_has... }
   { move=>Γ A B s r t tyA ihA tyB ihB Γ' ξ agr. asimpl.
     apply: sta_pi0... }
   { move=>Γ A B s r t tyA ihA tyB ihB Γ' ξ agr. asimpl.
@@ -84,7 +84,7 @@ Qed.
 
 Lemma sta_wf_ok Γ x A :
   sta_wf Γ -> sta_has Γ x A -> exists s, Γ ⊢ A : @s.
-Proof with eauto using agree_ren, agree_ren_refl.
+Proof with eauto using sta_agree_ren, sta_agree_ren_refl.
   move=>wf. elim: wf x A=>{Γ}.
   { move=>x A hs. inv hs. }
   { move=>Γ A s wf ih tyA x B hs. inv hs.
@@ -99,7 +99,7 @@ Qed.
 
 Lemma sta_weaken Γ m A B :
   Γ ⊢ m : A -> (B :: Γ) ⊢ m.[ren (+1)] : A.[ren (+1)].
-Proof with eauto using agree_ren, agree_ren_refl.
+Proof with eauto using sta_agree_ren, sta_agree_ren_refl.
   move=>ty. apply: sta_rename...
 Qed.
 
@@ -107,6 +107,6 @@ Lemma sta_eweaken Γ m m' A A' B :
   m' = m.[ren (+1)] ->
   A' = A.[ren (+1)] ->
   Γ ⊢ m : A -> (B :: Γ) ⊢ m' : A'.
-Proof with eauto using agree_ren, agree_ren_refl.
+Proof with eauto using sta_agree_ren, sta_agree_ren_refl.
   move=>*; subst. by apply: sta_weaken.
 Qed.
