theories/dyn_valid.v
@@ -1,0 +1,28 @@
+From mathcomp Require Import ssreflect ssrbool eqtype ssrnat seq.
+From Coq Require Import ssrfun Classical Utf8.
+Require Export AutosubstSsr ARS sta_valid dyn_type.
+
+Set Implicit Arguments.
+Unset Strict Implicit.
+Unset Printing Implicit Defensive.
+
+
+Lemma dyn_sta_type Γ Δ m A : Γ ; Δ ⊨ m : A -> Γ ⊢ m : A.
+Proof with eauto using sta_type.
+  move=>ty. elim: ty...
+Qed.
+
+Lemma dyn_sta_wf Γ Δ : dyn_wf Γ Δ -> sta_wf Γ.
+Proof with eauto using sta_wf.
+  move=>wf. elim: wf...
+Qed.
+
+Theorem dyn_valid Γ Δ m A :
+  dyn_wf Γ Δ -> Γ ; Δ ⊨ m : A -> exists s, Γ ⊢ A : @s.
+Proof.
+  move=>wf ty.
+  apply: sta_valid.
+  apply: dyn_sta_wf; eauto.
+  apply: dyn_sta_type; eauto.
+Qed.
+
