theories/dyn_weak.v
@@ -1,0 +1,99 @@
+From mathcomp Require Import ssreflect ssrbool eqtype ssrnat seq.
+From Coq Require Import ssrfun Classical Utf8.
+Require Export AutosubstSsr ARS sta_weak dyn_type.
+
+Set Implicit Arguments.
+Unset Strict Implicit.
+Unset Printing Implicit Defensive.
+
+Inductive dyn_agree_ren : (var -> var) ->
+  sta_ctx term -> dyn_ctx term -> sta_ctx term -> dyn_ctx term -> Prop :=
+| dyn_agree_ren_nil ξ :
+  dyn_agree_ren ξ nil nil nil nil
+| dyn_agree_ren_ty Γ Γ' Δ Δ' ξ m s :
+  dyn_agree_ren ξ Γ Δ Γ' Δ' ->
+  dyn_agree_ren (upren ξ)
+    (m :: Γ) (m :{s} Δ) (m.[ren ξ] :: Γ) (m.[ren ξ] :{s} Δ')
+| dyn_agree_ren_n Γ Γ' Δ Δ' ξ m :
+  dyn_agree_ren ξ Γ Δ Γ' Δ' ->
+  dyn_agree_ren (upren ξ)
+    (m :: Γ) (_: Δ) (m.[ren ξ] :: Γ) (_: Δ')
+| dyn_agree_ren_wkU Γ Γ' Δ Δ' ξ m :
+  dyn_agree_ren ξ Γ Δ Γ' Δ' ->
+  dyn_agree_ren (ξ >>> (+1)) Γ Δ (m :: Γ') (m :U Δ')
+| dyn_agree_ren_wkN Γ Γ' Δ Δ' ξ m :
+  dyn_agree_ren ξ Γ Δ Γ' Δ' ->
+  dyn_agree_ren (ξ >>> (+1)) Γ Δ (m :: Γ') (_: Δ').
+
+Lemma dyn_agree_ren_refl Γ Δ :
+  dyn_wf Γ Δ -> dyn_agree_ren id Γ Δ Γ Δ.
+Proof with eauto using dyn_agree_ren.
+  elim: Γ Δ.
+  { move=>Δ wf. inv wf... }
+  { move=>A Γ ih Δ wf. inv wf.
+    have agr:=ih _ H1.
+    have:dyn_agree_ren (upren id)
+      (A :: Γ) (A :{s} Δ0) (A.[ren id] :: Γ) (A.[ren id] :{s} Δ0)...
+    by asimpl. }
+Qed.
+
+Lemma dyn_agree_ren_key Γ Γ' Δ Δ' ξ s :
+  dyn_agree_ren ξ Γ Δ Γ' Δ' -> Δ ▷ s -> Δ' ▷ s.
+Proof with eauto using key.
+  move=>agr. elim: agr s=>{Γ Γ' Δ Δ' ξ}...
+  { move=>Γ Γ' Δ Δ' ξ m s agr ih t k. inv k... }
+  { move=>Γ Γ' Δ Δ' ξ _ agr ih s k. inv k... }
+  { move=>Γ Γ' Δ Δ' ξ m agr ih [] /ih... }
+Qed.
+
+Lemma dyn_agree_ren_has Γ Γ' Δ Δ' ξ x A :
+  dyn_agree_ren ξ Γ Δ Γ' Δ' -> dyn_has Δ x A -> dyn_has Δ' (ξ x) A.[ren ξ].
+Proof with eauto using dyn_agree_ren_key.
+  move=>agr. elim: agr x A=>{Γ Γ' Δ Δ' ξ}.
+  { move=>ξ x A hs. inv hs. }
+  { move=>Γ Γ' Δ Δ' ξ m s agr ih x A hs. inv hs; asimpl.
+    { replace m.[ren (ξ >>> (+1))] with m.[ren ξ].[ren (+1)] by autosubst.
+      constructor... }
+    { replace A0.[ren (ξ >>> (+1))] with A0.[ren ξ].[ren (+1)] by autosubst.
+      constructor... } }
+  { move=>Γ Γ' Δ Δ' ξ _ agr ih x A hs. inv hs; asimpl.
+    replace A0.[ren (ξ >>> (+1))] with A0.[ren ξ].[ren (+1)] by autosubst.
+     constructor... }
+  { move=>Γ Γ' Δ Δ' ξ m agr ih x A hs.
+    replace A.[ren (ξ >>> (+1))] with A.[ren ξ].[ren (+1)] by autosubst.
+    constructor... }
+  { move=>Γ Γ' Δ Δ' ξ _ agr ih x A hs.
+    replace A.[ren (ξ >>> (+1))] with A.[ren ξ].[ren (+1)] by autosubst.
+    constructor... }
+Qed.
+
+Lemma dyn_agree_ren_merge Γ Γ' Δ Δ' Δ1 Δ2 ξ :
+  dyn_agree_ren ξ Γ Δ Γ' Δ' -> Δ1 ∘ Δ2 => Δ ->
+  ∃ Δ1' Δ2',
+    Δ1' ∘ Δ2' => Δ' /\
+    dyn_agree_ren ξ Γ Δ1 Γ' Δ1' /\
+    dyn_agree_ren ξ Γ Δ2 Γ' Δ2'.
+Proof with eauto 6 using merge, dyn_agree_ren.
+  move=>agr. elim: agr Δ1 Δ2=>{Γ Γ' Δ Δ' ξ}.
+  { move=>ξ Δ1 Δ2 mrg. inv mrg.
+    exists nil. exists nil... }
+  { move=>Γ Γ' Δ Δ' ξ m s agr ih Δ1 Δ2 mrg. inv mrg.
+    { have[Δ1'[Δ2'[mrg'[agr1 agr2]]]]:=ih _ _ H2.
+      exists (m.[ren ξ] :U Δ1').
+      exists (m.[ren ξ] :U Δ2')... }
+    { have[Δ1'[Δ2'[mrg'[agr1 agr2]]]]:=ih _ _ H2.
+      exists (m.[ren ξ] :L Δ1').
+      exists (_: Δ2')... }
+    { have[Δ1'[Δ2'[mrg'[agr1 agr2]]]]:=ih _ _ H2.
+      exists (_: Δ1').
+      exists (m.[ren ξ] :L Δ2')... } }
+  { move=>Γ Γ' Δ Δ' ξ m agr ih Δ1 Δ2 mrg. inv mrg.
+    have[Δ1'[Δ2'[mrg'[agr1 agr2]]]]:=ih _ _ H2.
+      exists (_: Δ1'). exists (_: Δ2')... }
+  { move=>Γ Γ' Δ Δ' ξ m agr ih Δ1 Δ2 mrg.
+    have[Δ1'[Δ2'[mrg'[agr1 agr2]]]]:=ih _ _ mrg.
+    exists (m :U Δ1'). exists (m :U Δ2')... }
+  { move=>Γ Γ' Δ Δ' ξ m agr ih Δ1 Δ2 mrg.
+    have[Δ1'[Δ2'[mrg'[agr1 agr2]]]]:=ih _ _ mrg.
+    exists (_: Δ1'). exists (_: Δ2')... }
+Qed.
